code/experimental/rsa/Exponentiation.fst
@@ -1,86 +1,152 @@
 module Exponentiation
 
 open FStar.HyperStack.All
-open FStar.Buffer
+open Spec.Lib.IntBuf.Lemmas
+open Spec.Lib.IntBuf
+open Spec.Lib.IntTypes
+open FStar.Mul
 
 open Lib
 open Convert
 open Montgomery
 open Multiplication
 
-module U32 = FStar.UInt32
-module U64 = FStar.UInt64
-open U32
+module Buffer = Spec.Lib.IntBuf
 
 val mul_mod_mont:
-    exp_r:U32.t ->
-    rLen:U32.t -> r:lbignum rLen ->
-    n:lbignum rLen -> nInv:lbignum rLen ->
+    #rLen:size_nat ->
+    exp_r:size_t{v exp_r > 0} ->
+    rrLen:size_t{v rrLen == rLen /\ 6 * rLen < max_size_t} -> 
+    st_mont:lbignum (3 * rLen) ->
     aM:lbignum rLen -> bM:lbignum rLen ->
     resM:lbignum rLen -> Stack unit
-    (requires (fun h -> True))
-    (ensures (fun h0 _ h1 -> True))
+    (requires (fun h -> live h st_mont /\ live h aM /\ live h bM /\ live h resM))
+    (ensures (fun h0 _ h1 -> preserves_live h0 h1 /\ modifies1 resM h0 h1))
 
-let mul_mod_mont exp_r rLen r n nInv aM bM resM =
-    push_frame();
-    let c = create 0uL (rLen +^ rLen) in
-    bn_mul rLen aM rLen bM c; // c = a * b
-    mont_reduction exp_r rLen r n nInv c resM; // resM = c % n
-    pop_frame()
-
+let mul_mod_mont #rLen exp_r rrLen st_mont aM bM resM =
+    let cLen:size_t = add_mod #SIZE rrLen rrLen in
+    alloc #uint64 #unit #(v cLen) cLen (u64 0) [BufItem st_mont; BufItem aM; BufItem bM] [BufItem resM]
+    (fun h0 _ h1 -> True)
+    (fun c ->
+       bn_mul rrLen aM rrLen bM c; // c = a * b
+       mont_reduction exp_r rrLen st_mont cLen c resM // resM = c % n
+    )
+   
 val mod_exp_:
-    exp_r:U32.t ->
-    rLen:U32.t -> r:lbignum rLen ->
-    n:lbignum rLen -> nInv:lbignum rLen -> aM:lbignum rLen ->
-    bBits:U32.t{U32.v bBits > 0} -> bLen:U32.t{v bLen = v (bits_to_bn bBits)} -> b:lbignum bLen ->
-    accM:lbignum rLen -> count:U32.t{v count <= v bBits} -> Stack unit
-    (requires (fun h -> True))
-    (ensures  (fun h0 _ h1 -> True))
+    #rLen:size_nat -> #bLen:size_nat ->
+    exp_r:size_t{v exp_r > 0} ->
+    rrLen:size_t{v rrLen == rLen /\ 6 * rLen < max_size_t} -> 
+    st_mont:lbignum (3 * rLen) -> 
+    st_exp:lbignum (2 * rLen) ->
+    bBits:size_t{v bBits > 0} -> bbLen:size_t{v bbLen == bLen /\ bLen = v (bits_to_bn bBits)} -> b:lbignum bLen ->
+    count:size_t{v count <= v bBits} -> Stack unit
+    (requires (fun h -> live h st_mont /\ live h st_exp /\ live h b))
+    (ensures  (fun h0 _ h1 -> preserves_live h0 h1 /\ modifies1 st_exp h0 h1))
 
-let rec mod_exp_ exp_r rLen r n nInv aM bBits bLen b accM count =
-    if (count <^ bBits) then begin
-        (if (bn_is_bit_set bLen b count) then
-            mul_mod_mont exp_r rLen r n nInv aM accM accM); //acc = (acc * a) % n
-        mul_mod_mont exp_r rLen r n nInv aM aM aM; //a = (a * a) % n
-        mod_exp_ exp_r rLen r n nInv aM bBits bLen b accM U32.(count +^ 1ul)
+#reset-options "--z3rlimit 50 --max_fuel 0 --max_ifuel 0 "
+
+let rec mod_exp_ #rLen #bLen exp_r rrLen st_mont st_exp bBits bbLen b count =
+    let aM = Buffer.sub #uint64 #(rLen + rLen) #rLen st_exp (size 0) rrLen in
+    let accM = Buffer.sub #uint64 #(rLen + rLen) #rLen st_exp rrLen rrLen in
+    if (count <. bBits) then begin
+	assume (v count / 64 < bLen);
+        (if (bn_is_bit_set bbLen b count) then begin
+            mul_mod_mont exp_r rrLen st_mont aM accM accM end); //acc = (acc * a) % n
+        mul_mod_mont exp_r rrLen st_mont aM aM aM; //a = (a * a) % n
+	mod_exp_ exp_r rrLen st_mont st_exp bBits bbLen b (size_incr count)
     end
 
+val mod_exp_mont:
+    #rLen:size_nat -> #stLen:size_nat ->
+    bBits:size_t{0 < v bBits} -> b:lbignum (v (bits_to_bn bBits)) ->
+    exp_r:size_t{0 < v exp_r} -> rrLen:size_t{v rrLen == rLen} ->
+    sstLen:size_t{v sstLen == stLen /\ stLen = 9 * rLen} -> st:lbignum stLen -> Stack unit
+    (requires (fun h -> live h b /\ live h st /\ disjoint st b))
+    (ensures (fun h0 _ h1 -> preserves_live h0 h1 /\ modifies1 st h0 h1))
+
+#reset-options "--z3rlimit 150 --max_fuel 0 --max_ifuel 0"
+
+let mod_exp_mont #rLen #stLen bBits b exp_r rrLen sstLen st =
+    let bLen = bits_to_bn bBits in
+    
+    let r = Buffer.sub #uint64 #stLen #rLen st (size 0) rrLen in
+    let n1 = Buffer.sub #uint64 #stLen #rLen st rrLen rrLen in
+    let nInv = Buffer.sub #uint64 #stLen #rLen st (mul_mod #SIZE (size 2) rrLen) rrLen in
+    let r2 = Buffer.sub #uint64 #stLen #rLen st (mul_mod #SIZE (size 3) rrLen) rrLen in
+    
+    let a1 = Buffer.sub #uint64 #stLen #rLen st (mul_mod #SIZE (size 4) rrLen) rrLen in
+    let acc = Buffer.sub #uint64 #stLen #rLen st (mul_mod #SIZE (size 5) rrLen) rrLen in
+    let aM = Buffer.sub #uint64 #stLen #rLen st (mul_mod #SIZE (size 6) rrLen) rrLen in
+    let accM = Buffer.sub #uint64 #stLen #rLen st (mul_mod #SIZE (size 7) rrLen) rrLen in
+    let res1 = Buffer.sub #uint64 #stLen #rLen st (mul_mod #SIZE (size 8) rrLen) rrLen in
+    
+    let st_mont = Buffer.sub #uint64 #stLen #(3 * rLen) st (size 0) (mul_mod #SIZE (size 3) rrLen) in
+    let st_exp = Buffer.sub #uint64 #stLen #(2 * rLen) st (mul_mod #SIZE (size 6) rrLen) (mul_mod #SIZE (size 2) rrLen) in
+
+    to_mont exp_r rrLen st_mont r2 a1 aM;
+    to_mont exp_r rrLen st_mont r2 acc accM;
+
+    mod_exp_ exp_r rrLen st_mont st_exp bBits bLen b (size 0);
+
+    from_mont exp_r rrLen st_mont accM res1
+    
 // res = a ^^ b mod n
 val mod_exp:
-    modBits:U32.t{U32.v modBits > 0} ->
-    nLen:U32.t -> n:lbignum nLen -> a:lbignum nLen ->
-    bBits:U32.t{U32.v bBits > 0} -> b:lbignum (bits_to_bn bBits) ->
+    #nLen:size_nat ->
+    modBits:size_t{0 < v modBits /\ v modBits + 3 < max_size_t} ->
+    nnLen:size_t{v nnLen == nLen /\ 0 < nLen /\ nLen = v (bits_to_bn modBits)} ->
+    n:lbignum nLen -> a:lbignum nLen ->
+    bBits:size_t{0 < v bBits} -> b:lbignum (v (bits_to_bn bBits)) ->
     res:lbignum nLen -> Stack unit
-    (requires (fun h -> True))
-    (ensures  (fun h0 _ h1 -> True))
+    (requires (fun h -> live h n /\ live h a /\ live h b /\ live h res))
+    (ensures  (fun h0 _ h1 -> preserves_live h0 h1 /\ modifies1 res h0 h1))
+    
+#reset-options "--z3rlimit 50 --max_fuel 0 --max_ifuel 0"
 
-let mod_exp modBits nLen n a bBits b res =
-    push_frame();
-    let bLen = bits_to_bn bBits in
-    let rLen = bits_to_bn (3ul +^ modBits) in
-    let exp_r = modBits +^ 2ul in
-
-    let n1 = create 0uL rLen in
-    let a1 = create 0uL rLen in
-    let acc = create 0uL rLen in
-    let r = create 0uL rLen in
-    let r2 = create 0uL rLen in
-    let nInv = create 0uL rLen in
-    let aM = create 0uL rLen in
-    let accM = create 0uL rLen in
-    let res1 = create 0uL rLen in
-
-    blit n 0ul n1 0ul nLen;
-    blit a 0ul a1 0ul nLen;
-    acc.(0ul) <- 1uL;
-    bn_set_bit rLen r exp_r; // r = pow2 (2 + modBits)
-    bn_pow2_mod_n modBits rLen n1 (exp_r +^ exp_r) r2; // r2 = r * r % n
-    mont_inverse rLen n1 exp_r nInv; // n * nInv = 1 (mod r)
-    to_mont exp_r rLen r n1 nInv r2 a1 aM;
-    to_mont exp_r rLen r n1 nInv r2 acc accM;
-
-    mod_exp_ exp_r rLen r n1 nInv aM bBits bLen b accM 0ul;
-
-    from_mont exp_r rLen r n1 nInv accM res1;
-    blit res1 0ul res 0ul nLen;
-    pop_frame()
+let mod_exp #nLen modBits nnLen n a bBits b res =    
+    let exp_r:size_t = add #SIZE modBits (size 2) in
+    let rBits:size_t = add #SIZE modBits (size 3) in
+    let rLen = bits_to_bn rBits in
+    assume (nLen < v rLen);
+    assume (9 * v rLen < max_size_t);
+    assume (v exp_r / 64 < v rLen);
+    assume (v modBits / 64 < v rLen);
+    assume (v exp_r + v exp_r < max_size_t);
+    let stLen:size_t = mul #SIZE (size 9) rLen in
+    let stMLen:size_t = mul #SIZE (size 3) rLen in
+    let exp2:size_t = add #SIZE exp_r exp_r in
+    
+    alloc #uint64 #unit #(v stLen) stLen (u64 0) [BufItem n; BufItem a; BufItem b] [BufItem res]
+    (fun h0 _ h1 -> True)
+    (fun st ->
+      let r = Buffer.sub #uint64 #(v stLen) #(v rLen) st (size 0) rLen in
+      let n1 = Buffer.sub #uint64 #(v stLen) #(v rLen) st rLen rLen in
+      let nInv = Buffer.sub #uint64 #(v stLen) #(v rLen) st (mul #SIZE (size 2) rLen) rLen in
+      let r2 = Buffer.sub #uint64 #(v stLen) #(v rLen) st (mul #SIZE (size 3) rLen) rLen in
+      let a1 = Buffer.sub #uint64 #(v stLen) #(v rLen) st (mul #SIZE (size 4) rLen) rLen in
+      let acc = Buffer.sub #uint64 #(v stLen) #(v rLen) st (mul #SIZE (size 5) rLen) rLen in
+      //let aM = Buffer.sub #uint64 #(v stLen) #(v rLen) st (mul #SIZE (size 6) rLen) rLen in
+      //let accM = Buffer.sub #uint64 #(v stLen) #(v rLen) st (mul #SIZE (size 7) rLen) rLen in
+      let res1 = Buffer.sub #uint64 #(v stLen) #(v rLen) st (mul #SIZE (size 8) rLen) rLen in
+      //let st_mont = Buffer.sub #uint64 #(v stLen) #(3 * v rLen) st (size 0) (mul #SIZE (size 3) rLen) in
+      //let st_exp = Buffer.sub #uint64 #(v stLen) #(2 * v rLen) st (mul #SIZE (size 6) rLen) (mul #SIZE (size 2) rLen) in
+      
+      let n1_ = Buffer.sub #uint64 #(v rLen) #nLen n1 (size 0) nnLen in
+      let a1_ = Buffer.sub #uint64 #(v rLen) #nLen a1 (size 0) nnLen in
+      let res1_ = Buffer.sub #uint64 #(v rLen) #nLen res1 (size 0) nnLen in
+      
+      copy nnLen n n1_;
+      copy nnLen a a1_;
+      acc.(size 0) <- u64 1;
+      bn_set_bit rLen r exp_r; // r = pow2 (2 + modBits)
+      assume (disjoint r2 n1);
+      bn_pow2_mod_n modBits rLen n1 exp2 r2; // r2 = r * r % n
+      mont_inverse rLen n1 exp_r nInv; // n * nInv = 1 (mod r)
+      let h0 = FStar.HyperStack.ST.get() in
+      assert (live h0 st /\ live h0 b /\ disjoint st b);
+      mod_exp_mont #(v rLen) #(v stLen) bBits b exp_r rLen stLen st;
+      let h1 = FStar.HyperStack.ST.get() in
+      assert (preserves_live h0 h1 /\ modifies1 st h0 h1);
+      
+      copy nnLen res1_ res
+    )
