code/experimental/rsa/Multiplication.fst
@@ -1,75 +1,84 @@
 module Multiplication
 
 open FStar.HyperStack.All
-open FStar.Buffer
+open Spec.Lib.IntBuf.Lemmas
+open Spec.Lib.IntBuf
+open Spec.Lib.IntTypes
+
 open Lib
 
-module U32 = FStar.UInt32
-module U64 = FStar.UInt64
-module U128 = FStar.UInt128
-open U32
+module Buffer = Spec.Lib.IntBuf
 
 val bn_mul_by_limb_addj_f:
-    a_i:U64.t -> l:U64.t -> c:U64.t -> r_ij:U64.t -> Tot (tuple2 U64.t U64.t)
+    a_i:uint64 -> l:uint64 -> c:uint64 -> r_ij:uint64 -> Tot (tuple2 uint64 uint64)
+[@ "substitute"]    
 let bn_mul_by_limb_addj_f a_i l c r_ij =
-    let res = U128.(mul_wide a_i l +^ uint64_to_uint128 c +^ uint64_to_uint128 r_ij) in
-    let r = U128.uint128_to_uint64 res in
-    let c' = U128.shift_right res 64ul in
-    let c' = U128.uint128_to_uint64 c' in
+    //let res = (mul_wide a_i l) +. to_u128 c +. to_u128 r_ij in
+    let res = add_mod #U128 (to_u128 #U64 c) (to_u128 #U64 r_ij) in
+    let res = add_mod #U128 (mul_wide a_i l) res in
+    let r = to_u64 res in
+    let c' =  res >>. u32 64 in
+    let c' = to_u64 c' in
     (c', r)
 
 val bn_mul_by_limb_addj_:
-    aLen:U32.t -> a:lbignum aLen ->
-    l:U64.t -> i:U32.t{v i <= v aLen} -> j:U32.t ->
-    resLen:U32.t{v aLen + v j < v resLen} ->
-    res:lbignum resLen -> Stack U64.t
-    (requires (fun h -> True))
-    (ensures  (fun h0 _ h1 -> True))
-let rec bn_mul_by_limb_addj_ aLen a l i j resLen res =
-    if i =^ 0ul then 0uL
+    #aLen:size_nat -> #resLen:size_nat ->
+    caLen:size_t{v caLen == aLen} -> a:lbignum aLen ->
+    l:uint64 -> i:size_t{v i <= aLen} -> j:size_t ->
+    cresLen:size_t{aLen + v j < resLen} ->
+    res:lbignum resLen -> Stack uint64
+    (requires (fun h -> live h a /\ live h res /\ disjoint res a))
+    (ensures  (fun h0 _ h1 -> preserves_live h0 h1 /\ modifies1 res h0 h1))
+    
+let rec bn_mul_by_limb_addj_ #aLen #resLen caLen a l i j cresLen res =
+    if i =. size 0 then u64 0
     else begin
-        let i1 = i -^ 1ul in
-        let c1 = bn_mul_by_limb_addj_ aLen a l i1 j resLen res in
-        let (carry', res_ij) = bn_mul_by_limb_addj_f a.(i1) l c1 res.(i1 +^ j) in
-        res.(i1 +^ j) <- res_ij;
+        let i1 = size_decr i in
+        let c1 = bn_mul_by_limb_addj_ #aLen #resLen caLen a l i1 j cresLen res in
+        let (carry', res_ij) = bn_mul_by_limb_addj_f a.(i1) l c1 res.(add_mod #SIZE i1 j) in
+        res.(add_mod #SIZE i1 j) <- res_ij;
         carry'
     end
 
 val bn_mul_by_limb_addj:
-    aLen:U32.t -> a:lbignum aLen -> l:U64.t -> j:U32.t ->
-    resLen:U32.t{v aLen + v j < v resLen} ->
-    res:lbignum resLen -> Stack U64.t
-    (requires (fun h -> True))
-    (ensures  (fun h0 _ h1 -> True))
+    #aLen:size_nat -> #resLen:size_nat ->
+    caLen:size_t{v caLen == aLen} -> a:lbignum aLen -> l:uint64 -> j:size_t ->
+    cresLen:size_t{aLen + v j < resLen} ->
+    res:lbignum resLen -> Stack uint64
+    (requires (fun h -> live h a /\ live h res /\ disjoint res a))
+    (ensures  (fun h0 _ h1 -> preserves_live h0 h1 /\ modifies1 res h0 h1))
 
-let bn_mul_by_limb_addj aLen a l j resLen res =
-    bn_mul_by_limb_addj_ aLen a l aLen j resLen res
+[@ "substitute"]
+let bn_mul_by_limb_addj #aLen #resLen caLen a l j cresLen res =
+    bn_mul_by_limb_addj_ #aLen #resLen caLen a l caLen j cresLen res
 
 val bn_mul_:
-    aLen:U32.t -> a:lbignum aLen ->
-    bLen:U32.t -> b:lbignum bLen ->
-    j:U32.t{v j <= v bLen} ->
-    resLen:U32.t{v resLen = v aLen + v bLen} ->
+    #aLen:size_nat -> #bLen:size_nat -> #resLen:size_nat ->
+    caLen:size_t{v caLen == aLen} -> a:lbignum aLen ->
+    cbLen:size_t{v cbLen == bLen} -> b:lbignum bLen ->
+    j:size_t{v j <= bLen} ->
+    cresLen:size_t{v cresLen == resLen /\  resLen = aLen + bLen} ->
     res:lbignum resLen -> Stack unit
-    (requires (fun h -> True))
-    (ensures  (fun h0 _ h1 -> True))
+    (requires (fun h -> live h a /\ live h b /\ live h res /\ disjoint res a /\ disjoint res b))
+    (ensures  (fun h0 _ h1 -> preserves_live h0 h1 /\ modifies1 res h0 h1))
 
-let rec bn_mul_ aLen a bLen b j resLen res =
-    if j =^ 0ul then ()
+let rec bn_mul_ #aLen #bLen #resLen caLen a cbLen b j cresLen res =
+    if j =. size 0 then ()
     else begin
-        let j1 = j -^ 1ul in
-        bn_mul_ aLen a bLen b j1 resLen res;
-        let c' = bn_mul_by_limb_addj aLen a b.(j1) j1 resLen res in
-        res.(aLen +^ j1) <- c'
+        let j1 = size_decr j in
+        bn_mul_ #aLen #bLen #resLen caLen a cbLen b j1 cresLen res;
+        let c' = bn_mul_by_limb_addj #aLen #resLen caLen a b.(j1) j1 cresLen res in
+        res.(add_mod #SIZE caLen j1) <- c'
     end
 
 // res = a * b
 val bn_mul:
-    aLen:U32.t -> a:lbignum aLen ->
-    bLen:U32.t -> b:lbignum bLen ->
-    res:lbignum (aLen +^ bLen) -> Stack unit
-    (requires (fun h -> True))
-    (ensures  (fun h0 _ h1 -> True))
+    #aLen:size_nat -> #bLen:size_nat ->
+    caLen:size_t{v caLen == aLen} -> a:lbignum aLen ->
+    cbLen:size_t{v cbLen == bLen /\ aLen + bLen < max_size_t} -> b:lbignum bLen ->
+    res:lbignum (aLen + bLen) -> Stack unit
+    (requires (fun h -> live h a /\ live h b /\ live h res /\ disjoint res a /\ disjoint res b))
+    (ensures  (fun h0 _ h1 -> preserves_live h0 h1 /\ modifies1 res h0 h1))
         
-let bn_mul aLen a bLen b res = 
-    bn_mul_ aLen a bLen b bLen (aLen +^ bLen) res
+let bn_mul #aLen #bLen caLen a cbLen b res = 
+    bn_mul_ #aLen #bLen #(aLen + bLen) caLen a cbLen b cbLen (add_mod #SIZE caLen cbLen) res
