code/experimental/rsa/Shift.fst
@@ -1,157 +1,108 @@
 module Shift
 
 open FStar.HyperStack.All
-open FStar.Buffer
-open FStar.Int.Cast
+open Spec.Lib.IntBuf.Lemmas
+open Spec.Lib.IntBuf
+open Spec.Lib.IntTypes
 
 open Lib
-open Addition
 
-module U32 = FStar.UInt32
-module U64 = FStar.UInt64
-open U32
+module Buffer = Spec.Lib.IntBuf
 
-let bn_tbit = 0x8000000000000000uL
-
-val bn_lshift_:
-    aLen:U32.t -> a:lbignum aLen ->
-    count:U32.t -> nw:U32.t ->
-    lb:U32.t{0 < v lb /\ v lb < 64} ->
-    res:lbignum aLen{v count + v nw < v aLen} -> Stack unit
-	(requires (fun h -> True))
-	(ensures (fun h0 _ h1 -> True))
-let rec bn_lshift_ aLen a count nw lb res =
-    if count >^ 0ul then begin
-        let i = nw +^ count in
-        let tmp = res.(i) in
-        let count = count -^ 1ul in
-        let t1 = a.(count) in
-        let rb = 64ul -^ lb in
-        assert(0 < v rb /\ v rb < 64);
-        res.(i) <- U64.(tmp |^ U64.(t1 >>^ rb));
-        res.(i -^ 1ul) <- U64.(t1 <<^ lb);
-        bn_lshift_ aLen a count nw lb res end
-
-(* res = a << n *)
-val bn_lshift:
-    aLen:U32.t -> a:lbignum aLen ->
-    nCount:U32.t{v nCount > 0 /\ v aLen - (v nCount) / 64 - 1 > 0} ->
-    res:lbignum aLen -> Stack unit
-	(requires (fun h -> True))
-	(ensures (fun h0 _ h1 -> True))
-let bn_lshift aLen a nCount res =
-    let nw = nCount /^ 64ul in
-    let lb = nCount %^ 64ul in
-    (if lb =^ 0ul then
-        blit a 0ul res nw (aLen -^ nw)
-    else bn_lshift_ aLen a (aLen -^ nw -^ 1ul) nw lb res)
-
+let bn_tbit = u64 0x8000000000000000
 
 val bn_lshift1_:
-    aLen:U32.t -> a:lbignum aLen ->
-    carry:U64.t -> i:U32.t{v i < v aLen} ->
+    #aLen:size_nat ->
+    caLen:size_t{v caLen == aLen} -> a:lbignum aLen ->
+    carry:uint64 -> i:size_t{v i <= aLen} ->
     res:lbignum aLen -> Stack unit
-    (requires (fun h -> True))
-	(ensures (fun h0 _ h1 -> True))
-let rec bn_lshift1_ aLen a carry i res =
-    if i <^ aLen then begin
+    (requires (fun h -> live h a /\ live h res))
+    (ensures (fun h0 _ h1 -> preserves_live h0 h1 /\ modifies1 res h0 h1))
+
+let rec bn_lshift1_ #aLen caLen a carry i res =
+    if (i <. caLen) then begin
         let tmp = a.(i) in
-        res.(i) <- U64.((tmp <<^ 1ul) |^ carry);
-        let carry = if U64.((tmp &^ bn_tbit) =^ bn_tbit) then 1uL else 0uL in
-        bn_lshift1_ aLen a carry (i +^ 1ul) res end
+        res.(i) <- (shift_left #U64 tmp (u32 1)) |. carry;
+        let carry = if (eq_u64 (logand #U64 tmp bn_tbit) bn_tbit) then u64 1 else u64 0 in
+        bn_lshift1_ #aLen caLen a carry (size_incr i) res
+    end
 
 (* res = a << 1 *)
 val bn_lshift1:
-    aLen:U32.t -> a:lbignum aLen ->
+    #aLen:size_nat ->
+    caLen:size_t{v caLen == aLen} -> a:lbignum aLen ->
     res:lbignum aLen -> Stack unit
-	(requires (fun h -> True))
-	(ensures (fun h0 _ h1 -> True))
+    (requires (fun h -> live h a /\ live h res))
+    (ensures (fun h0 _ h1 -> preserves_live h0 h1 /\ modifies1 res h0 h1))
 
-let bn_lshift1 aLen a res = bn_lshift1_ aLen a 0uL 0ul res
-
+let bn_lshift1 #aLen caLen a res = bn_lshift1_ #aLen caLen a (u64 0) (size 0) res
 
 val bn_rshift_:
-    aLen:U32.t -> a:lbignum aLen ->
-    i:U32.t{v i > 0} -> nw:U32.t ->
-    rb:U32.t{0 < v rb /\ v rb < 64} -> l:U64.t ->
-    res:lbignum aLen{v i + v nw < v aLen} -> Stack unit
-	(requires (fun h -> True))
-	(ensures (fun h0 _ h1 -> True))
-let rec bn_rshift_ aLen a i nw rb l res =
-    if (i <^ aLen -^ nw) then begin
-        let tmp = U64.(l >>^ rb) in
-        let l = a.(nw +^ i) in
-        let lb = 64ul -^ rb in
-        assert(0 < v lb /\ v lb < 64);
-        res.(i -^ 1ul) <- U64.(tmp |^ U64.(l <<^ lb));
-        bn_rshift_ aLen a (i +^ 1ul) nw rb l res end
-    else res.(i -^ 1ul) <- U64.(l >>^ rb)
+    #aLen:size_nat ->
+    caLen:size_t{v caLen == aLen} -> a:lbignum aLen ->
+    i:size_t{v i > 0} -> nw:size_t ->
+    rb:uint32{0 < uint_v #U32 rb /\ uint_v #U32 rb < 64} -> l:uint64 ->
+    res:lbignum aLen{v i + v nw <= aLen} -> Stack unit
+    (requires (fun h -> live h a /\ live h res))
+    (ensures (fun h0 _ h1 -> preserves_live h0 h1 /\ modifies1 res h0 h1))
+
+#reset-options "--z3rlimit 50 --max_fuel 0"
+
+let rec bn_rshift_ #aLen caLen a i nw rb l res =
+    if (i <. sub_mod #SIZE caLen nw) then begin
+        let tmp = l >>. rb in
+        let l = a.(add_mod #SIZE nw i) in
+        let lb = u32 64 -. rb in
+        assert(0 < uint_v #U32 lb /\ uint_v #U32 lb < 64);
+        res.(size_decr i) <- tmp |. (shift_left #U64 l lb);
+        bn_rshift_ #aLen caLen a (size_incr i) nw rb l res end
+    else res.(size_decr i) <- shift_right #U64 l rb
 
 (* res = a >> n *)
 val bn_rshift:
-    aLen:U32.t -> a:lbignum aLen ->
-    nCount:U32.t{v nCount > 0 /\ v aLen - (v nCount) / 64 - 1 > 0} ->
+    #aLen:size_nat ->
+    caLen:size_t{v caLen == aLen} -> a:lbignum aLen ->
+    nCount:size_t{v nCount > 0 /\ aLen - v nCount / 64 - 1 > 0} ->
     res:lbignum aLen -> Stack unit
-	(requires (fun h -> True))
-	(ensures (fun h0 _ h1 -> True))
-let bn_rshift aLen a nCount res =
-    let nw = nCount /^ 64ul in
-    let rb = nCount %^ 64ul in
-    (if rb =^ 0ul then
-        blit a nw res 0ul (aLen -^ nw)
-    else
+    (requires (fun h -> live h a /\ live h res))
+    (ensures (fun h0 _ h1 -> preserves_live h0 h1 /\ modifies1 res h0 h1))
+	
+let bn_rshift #aLen caLen a nCount res =
+    let nw = nCount /. size 64 in
+    let rb = nCount %. size 64 in
+    (if rb =. size 0 then begin
+	let a_Len:size_t =sub_mod #SIZE caLen nw in
+	let a_ = Buffer.sub #uint64 #aLen #(v a_Len) a nw a_Len in
+	let res_ = Buffer.sub #uint64 #aLen #(v a_Len) res (size 0) a_Len in
+	copy a_Len a_ res_ end
+    else begin
         let l = a.(nw) in
-        bn_rshift_ aLen a 1ul nw rb l res)
-
-
-val bn_rshift1_:
-    aLen:U32.t -> a:lbignum aLen ->
-    carry:U64.t -> i:U32.t{v i < v aLen} ->
-    res:lbignum aLen -> Stack unit
-    (requires (fun h -> True))
-	(ensures (fun h0 _ h1 -> True))
-let rec bn_rshift1_ aLen a carry i res =
-    if i >^ 0ul then begin
-        let i = i -^ 1ul in
-        let tmp = a.(i) in
-        res.(i) <- U64.((tmp >>^ 1ul) |^ carry);
-        let carry = if U64.((tmp &^ 1uL) =^ 1uL) then bn_tbit else 0uL in
-        bn_rshift1_ aLen a carry i res end
-
-(* res = a >> 1 *)
-val bn_rshift1:
-    aLen:U32.t -> a:lbignum aLen ->
-    res:lbignum aLen -> Stack unit
-	(requires (fun h -> True))
-	(ensures (fun h0 _ h1 -> True))
-let bn_rshift1 aLen a res =
-    //if a is 0 then return 0
-    let i = aLen -^ 1ul in
-    let tmp = a.(i) in
-    let carry = if U64.((tmp &^ 1uL) =^ 1uL) then bn_tbit else 0uL in
-    let tmp = U64.(tmp >>^ 1ul) in
-    //(if U64.(tmp >^ 0uL) then res.(i) <- tmp);
-    res.(i) <- tmp;
-    bn_rshift1_ aLen a carry i res
+        bn_rshift_ #aLen caLen a (size 1) nw (size_to_uint32 rb) l res end)
 
 // res = a % (pow2 nCount)
 val bn_mod_pow2_n:
-    aLen:U32.t -> a:lbignum aLen ->
-    nCount:U32.t ->
-    resLen:U32.t -> res:lbignum resLen -> Stack unit
-	(requires (fun h -> True))
-	(ensures (fun h0 _ h1 -> True))
+    #aLen:size_nat -> #resLen:size_nat ->
+    caLen:size_t{v caLen == aLen} -> a:lbignum aLen ->
+    nCount:size_t ->
+    cresLen:size_t{v cresLen == resLen /\ resLen <= aLen /\ resLen - v nCount / 64 - 1 > 0} ->
+    res:lbignum resLen -> Stack unit
+    (requires (fun h -> live h a /\ live h res /\ disjoint res a))
+    (ensures (fun h0 _ h1 -> preserves_live h0 h1 /\ modifies1 res h0 h1))
 
-let bn_mod_pow2_n aLen a nCount resLen res =
-    let nw = nCount /^ 64ul in
-    let nb = nCount %^ 64ul in
-    blit a 0ul res 0ul resLen;
+let bn_mod_pow2_n #aLen #resLen caLen a nCount cresLen res =
+    let nw = nCount /. size 64 in
+    let nb = nCount %. size 64 in
+    let a_ = Buffer.sub a (size 0) cresLen in
+    copy cresLen a_ res;
 
-    let start_i =
-        if (nb >^ 0ul) then begin
-            res.(nw) <- U64.(res.(nw) &^ (0xffffffffffffffffuL >>^ U32.(64ul -^ nb)));
-            nw +^ 1ul end
+    let start_i:size_t =
+        if (nb >. size 0) then begin
+	    let lb = sub_mod #U32 (u32 64) (size_to_uint32 nb) in
+            res.(nw) <- res.(nw) &. (shift_right #U64 (u64 0xffffffffffffffff) lb);
+            size_incr nw end
         else nw in
 
-    let res' = Buffer.sub res start_i (resLen -^ start_i) in
-    fill res' 0uL (resLen -^ start_i)
+    let res_Len:size_t = sub_mod #SIZE cresLen start_i in
+    assume (v start_i + v res_Len <= resLen);
+    let res_ = Buffer.sub #uint64 #resLen #(v res_Len) res start_i res_Len in
+    fill res_Len res_ (u64 0)
