specs/lib/c/Spec.Lib.Endian.fst
@@ -8,3 +8,8 @@ open FStar.HyperStack.ST
 #reset-options "--z3rlimit 50"
 let uint32_from_bytes_le (i:lbuffer uint8 4) = C.load32_le i
 
+let uint64_from_bytes_be (i:lbuffer uint8 8) = C.load64_be i
+
+let uint64_to_bytes_be (i:lbuffer uint8 8) (z:uint64) = C.store64_be i z
+
+
