code/experimental/rsa/Comparison.fst
@@ -1,35 +1,35 @@
 module Comparison
 
 open FStar.HyperStack.All
-open FStar.Buffer
+open Spec.Lib.IntBuf.Lemmas
+open Spec.Lib.IntBuf
+open Spec.Lib.IntTypes
+
 open Lib
 
-module U32 = FStar.UInt32
-module U64 = FStar.UInt64
-open U32
-
 val bn_is_less_:
-    len:U32.t ->
+    #len:size_nat -> clen:size_t{v clen == len} ->
     a:lbignum len ->
     b:lbignum len ->
-    i:U32.t{v i <= v len} -> Stack bool
-    (requires (fun h -> True))
-    (ensures (fun h0 _ h1 -> True))
-let rec bn_is_less_ len a b i =
-    if (i >^ 0ul) then
-        let i = i -^ 1ul in
+    i:size_t{v i <= len} -> Stack bool
+    (requires (fun h -> live h a /\ live h b /\ disjoint a b))
+    (ensures (fun h0 _ h1 -> preserves_live h0 h1 /\ h0 == h1))
+
+let rec bn_is_less_ #len clen a b i =
+    if (i >. size 0) then
+        let i = size_decr i in
         let t1 = a.(i) in
         let t2 = b.(i) in
-        (if not (U64.(t1 =^ t2)) then
-            if U64.(t1 <^ t2) then true else false
-        else bn_is_less_ len a b i)
+        (if not (eq_u64 t1 t2) then
+            if lt_u64 t1 t2 then true else false
+        else bn_is_less_ #len clen a b i)
     else false
 
 (* if a < b then true else false *)
 val bn_is_less:
-    len:U32.t ->
+    #len:size_nat -> clen:size_t{v clen == len} ->
     a:lbignum len ->
     b:lbignum len -> Stack bool
-    (requires (fun h -> True))
-    (ensures (fun h0 _ h1 -> True))
-let bn_is_less len a b = bn_is_less_ len a b len
+    (requires (fun h -> live h a /\ live h b /\ disjoint a b))
+    (ensures (fun h0 _ h1 -> preserves_live h0 h1 /\ h0 == h1))
+let bn_is_less #len clen a b = bn_is_less_ #len clen a b clen
