specs/lib/Spec.Lib.Endian.fsti
@@ -9,4 +9,14 @@ val uint32_from_bytes_le: i:lbuffer uint8 4 -> Stack uint32
 			 (requires (fun h -> live h i))
 			 (ensures (fun h0 _ h1 -> preserves_live h0 h1 /\ h0 == h1))
 
+inline_for_extraction
+val uint64_from_bytes_be: i:lbuffer uint8 8 -> Stack uint64 
+			 (requires (fun h -> live h i))
+			 (ensures (fun h0 _ h1 -> preserves_live h0 h1 /\ h0 == h1))
+
+inline_for_extraction
+val uint64_to_bytes_be: i:lbuffer uint8 8 -> uint64 -> Stack unit
+			(requires (fun h -> live h i))
+			(ensures (fun h0 _ h1 -> preserves_live h0 h1 /\ h0 == h1))
+ 
 
